
\begin{theoremEnd}{theorem}\label{thm:thm_bias_diff}
  Assuming \(\eta\left(\vz\right) < M \, \pi\left(\vz\right)\) for some \(M < \infty\), when using the IMH kernel, the reduction in bias by using the sequential state estimator with \(N\) states instead of the parallel state estimator with \(N\) chains is bounded as
  {\small
  \begin{align*}
    &\abs{
      \text{Bias}\left[\vg_{\text{seq.-IMH}}\right]
      -
      \text{Bias}\left[\vg_{\text{par.-IMH}}\right]
    }
    \\
    &\quad\leq
    C_1 \, \max\left\{\, n \, {\left(1 - \frac{1}{w^*} \right)}^{n-1} - 1, 1 \,\right\}
    +
    C_2 \, \left( 1 - \frac{1}{w^*} \right)
  \end{align*}
  }
  for some positive constants \(C_1\) and \(C_2\).
\end{theoremEnd}
\begin{proofEnd}
  {\small
  \begin{align}
    &\abs{
      \text{Bias}\left[\vg_{\text{seq.-IMH}}\right]
      -
      \text{Bias}\left[\vg_{\text{par.-IMH}}\right]
    }
    \\
    &\leq
    \norm{
      \int \eta\left(\vz\right) \int \frac{1}{N} \sum_{n=1}^{N} K^n\left(\vz, \vz^*\right) \vs\left(\vlambda;\vz^*\right) d\vz^* \, d\vz
      -
      \int \eta\left(\vz\right) \int \frac{1}{N} \sum_{n=1}^{N} K\left(\vz^{(n)}, \vz^*\right) \vs\left(\vlambda;\vz^*\right) d\vz^* \, d\vz_{(1:N)}
    }&\text{\footnotesize(Triangle Inequality)}
    \\
    &=
    \norm{
      \int \eta\left(\vz\right) \int \frac{1}{N} \sum_{n=1}^{N} K^n\left(\vz, \vz^*\right) \vs\left(\vlambda;\vz^*\right) d\vz^* \, d\vz
      -
      \int \eta\left(\vz\right) \int \frac{1}{N} \sum_{n=1}^{N} K\left(\vz, \vz^*\right) \vs\left(\vlambda;\vz^*\right) d\vz^* \, d\vz
    }&\text{\footnotesize(Independence)}
    \\
    &=
    \norm{
      \int \eta\left(\vz\right) \int \frac{1}{N} \sum_{n=1}^{N} \left(K^n\left(\vz, \vz^*\right) - K\left(\vz, \vz^*\right) \right) \vs\left(\vlambda;\vz^*\right) d\vz^* \, d\vz
    }
    \\
    &\leq
    \frac{1}{N} \sum_{n=1}^{N} 
    \norm{
      \int \int \eta\left(\vz\right) \left(K^n\left(\vz, \vz^*\right) - K\left(\vz, \vz^*\right) \right) \vs\left(\vlambda;\vz^*\right) d\vz^* \, d\vz
    }&\text{\footnotesize(Triangle Inequality)}
    \\
    &=
    \frac{1}{N} \sum_{n=1}^{N}
    \Big\lVert\;
      \int \eta\left(\vz\right) \int \pi\left(\vz^*\right) \, \left(
      T_n\left(w\left(\vz\right) \vee w\left(\vz^*\right) \right) - T_1\left(w\left(\vz\right) \vee w\left(\vz^*\right) \right) \right)
      \vs\left(\vlambda;\vz^*\right) d\vz^* \, d\vz
      \nonumber
      \\
      &\quad\qquad\qquad +
      \int \eta\left(\vz\right) \left(\lambda^{n}\left( w\left(\vz\right) \right) - \lambda\left( w\left(\vz\right) \right)\right) \vs\left(\vlambda;\vz\right) \, d\vz
    \;\Big\rVert
    &\text{\footnotesize(\cref{thm:imh_exact_kernel})}
    \\
    &\leq
    \frac{1}{N} \sum_{n=1}^{N}
    \norm{
      \int \eta\left(\vz\right) \int \pi\left(\vz^*\right) \,
      \left( T_n\left(w\left(\vz\right) \vee w\left(\vz^*\right) \right) - T_1\left(w\left(\vz\right) \vee w\left(\vz^*\right) \right)\right)
      \vs\left(\vlambda;\vz^*\right) d\vz^* \, d\vz
    }
      \nonumber
      \\
      &\qquad +
      \frac{1}{N} \sum_{n=1}^{N}
      \norm{
        \int \eta\left(\vz\right) \left(\lambda^{n}\left( w\left(\vz\right) \right) - \lambda\left( w\left(\vz\right) \right)\right) \vs\left(\vlambda;\vz\right) \, d\vz
      }
      &\text{\footnotesize(Triangle Inequality)}
    \\
    &\leq
    \frac{1}{N} \sum_{n=1}^{N}
    \underbrace{
      \int \eta\left(\vz\right) \int \pi\left(\vz^*\right) \,
      \abs{ T_n\left(w\left(\vz\right) \vee w\left(\vz^*\right) \right) - T_1\left(w\left(\vz\right) \vee w\left(\vz^*\right) \right) } \;
      \norm{ \vs\left(\vlambda;\vz^*\right)} \, d\vz^* \, d\vz
    }_{T1}
      \nonumber
      \\
      &\qquad +
      \frac{1}{N} \sum_{n=1}^{N}
    \underbrace{
        \int \eta\left(\vz\right) \abs{ \lambda^{n}\left( w\left(\vz\right) \right) - \lambda\left( w\left(\vz\right) \right)} \; \norm{\vs\left(\vlambda;\vz\right)} \, d\vz
    }_{T2}\label{eq:bias_diff_bound_master}
  \end{align}
  }

  Now, denoting \(w^{\prime} = w\left(\vz\right) \vee w\left(\vz^*\right)\),
  \begin{align}
    \abs{ T_n\left(w\left(\vz\right) \vee w\left(\vz^*\right) \right) - T_1\left(w\left(\vz\right) \vee w\left(\vz^*\right) \right) }
    &=
    \abs{ \int_{w^{\prime}}^{\infty}  \frac{1}{v^2} \, n \, \lambda^{n-1}\left(w\left(\vz\right)\right) \, dv  - \int_{w^{\prime}}^{\infty}  \frac{1}{v^2} dv }
    \\
    &=
    \abs{ \int_{w^{\prime}}^{\infty}  \frac{1}{v^2} \left( n \, \lambda^{n-1}\left(w\left(\vz\right)\right) - 1 \right) \, dv }
    \\
    &\leq
    \int_{w^{\prime}}^{\infty}  \frac{1}{v^2} \, \abs{ n \, \lambda^{n-1}\left(w\left(\vz\right)\right) - 1 } \, dv.\label{eq:diff_T}
  \end{align}

  Since
  \[
  0 \leq \lambda\left(w\left(\vz\right)\right) \leq 1 - \frac{1}{w^*} \leq 1,
  \]
  if follows that
  \[
  -1 \leq n \, \lambda^{n-1}\left(w\left(\vz\right)\right) - 1 \leq n \, {\left(1 - \frac{1}{w^*}\right)}^{n-1} - 1,
  \]
  and thus
  \[
  \abs{ n \, \lambda^{n-1}\left(w\left(\vz\right)\right) - 1 } \leq \max\left\{\; n \, {\left(1 - \frac{1}{w^*}\right)}^{n-1} - 1, 1\;\right\}.
  \]

Then, we can bound~\cref{eq:diff_T} as
  \begin{align}
    \int_{w^{\prime}}^{\infty}  \frac{1}{v^2} \, \abs{ n \, \lambda^{n-1}\left(w\left(\vz\right)\right) - 1 } \, dv
    &\leq
    \int_{w^{\prime}}^{\infty}  \frac{1}{v^2} \, \max\left\{\, n \, {\left(1 - \frac{1}{w^*}\right)}^{n-1} - 1, 1 \,\right\}\, dv
    \\
    &=
    \max\left\{\, n \, {\left(1 - \frac{1}{w^*}\right)}^{n-1} - 1, 1 \,\right\}\,\int_{w^{\prime}}^{\infty}  \frac{1}{v^2}
    \\
    &=
    \max\left\{\, n \, {\left(1 - \frac{1}{w^*}\right)}^{n-1} - 1, 1 \,\right\} \, \frac{1}{w^{\prime}}
    \\
    &=
    \max\left\{\, n \, {\left(1 - \frac{1}{w^*}\right)}^{n-1} - 1, 1 \,\right\} \frac{1}{w\left(\vz\right) \vee w\left(\vz^*\right)}.
  \end{align}
  
  Now, back to~\cref{eq:bias_diff_bound_master}, T1 can be bounded as
  \begin{align}
    &\int \eta\left(\vz\right) \int \pi\left(\vz^*\right) \,
    \abs{ T_n\left(w\left(\vz\right) \vee w\left(\vz^*\right) \right) - T_1\left(w\left(\vz\right) \vee w\left(\vz^*\right) \right) } \;
    \norm{ \vs\left(\vlambda;\vz^*\right)} \, d\vz^* \, d\vz
    \\
    &\leq
    \int \eta\left(\vz\right) \int \pi\left(\vz^*\right) \,
    \max\left\{\, n \, {\left(1 - \frac{1}{w^*}\right)}^{n-1} - 1, 1 \,\right\}\,\frac{1}{w\left(\vz\right) \vee w\left(\vz^*\right)}\,
    \norm{ \vs\left(\vlambda;\vz^*\right)} \, d\vz^* \, d\vz
    \\
    &= \max\left\{\, n \, {\left(1 - \frac{1}{w^*}\right)}^{n-1} - 1, 1 \,\right\}  \nonumber
    \\ &\qquad
    \times
    \int \eta\left(\vz\right) \,
    \left\{\;
    \int_{A\left(w\left(\vz\right)\right)} \pi\left(\vz^*\right) \,
    \frac{1}{w\left(\vz^*\right)} \;
    \norm{ \vs\left(\vlambda;\vz^*\right)} \, d\vz^*
    +
    \int_{R\left(w\left(\vz\right)\right)} \pi\left(\vz^*\right) \,
    \frac{1}{w\left(\vz\right)} \;
    \norm{ \vs\left(\vlambda;\vz^*\right)} \, d\vz^*
    \;\right\}  \, d\vz
    \\
    &=
    \max\left\{\, n \, {\left(1 - \frac{1}{w^*}\right)}^{n-1} - 1, 1 \,\right\}  \nonumber
    \\
    &\qquad
    \times
    \left\{\;
    \underbrace{
    \int \eta\left(\vz\right) \int_{A\left(w\left(\vz\right)\right)} \pi\left(\vz^*\right) \,
    \frac{1}{w\left(\vz^*\right)} \;
    \norm{ \vs\left(\vlambda;\vz^*\right)} \, d\vz^* \, d\vz
    }_{T3}
    +
    \underbrace{
    \int \eta\left(\vz\right) \,
    \frac{1}{w\left(\vz\right)} \, d\vz \,
    \int_{R\left(w\left(\vz\right)\right)} \pi\left(\vz^*\right) \,
    \norm{ \vs\left(\vlambda;\vz^*\right)} \, d\vz^* \, d\vz
    }_{T4}
    \;\right\}.
  \end{align}

  T3 reduces to
  \begin{align}
    \int \eta\left(\vz\right) \int_{A\left(w\left(\vz\right)\right)} \pi\left(\vz^*\right) \,
    \frac{1}{w\left(\vz^*\right)} \;
    \norm{ \vs\left(\vlambda;\vz^*\right)} \, d\vz^* \, d\vz
    &\leq
    \int \eta\left(\vz\right) \int \pi\left(\vz^*\right) \,
    \frac{1}{w\left(\vz^*\right)} \;
    \norm{ \vs\left(\vlambda;\vz^*\right)} \, d\vz^* \, d\vz
    \\
    &=
    \int \eta\left(\vz\right) \, d\vz \, \int \pi\left(\vz^*\right) \,
    \frac{1}{w\left(\vz^*\right)} \;
    \norm{ \vs\left(\vlambda;\vz^*\right)} \, d\vz^* 
    \\
    &=
    \int \pi\left(\vz^*\right) \,
    \frac{1}{w\left(\vz^*\right)} \;
    \norm{ \vs\left(\vlambda;\vz^*\right)} \, d\vz^* 
    \\
    &=
    \int q\left(\vz^*\right) \, \norm{ \vs\left(\vlambda;\vz^*\right)} \, d\vz^* 
    \\
    &=
    \Esub{q}{\norm{ \vs\left(\vlambda;\vz^*\right)}},
  \end{align}
  which is a positive constant.

  On the other hand, T4 becomes
  \begin{align}
    \int \eta\left(\vz\right) \,
    \frac{1}{w\left(\vz\right)} \, d\vz \,
    \int_{R\left(w\left(\vz\right)\right)} \pi\left(\vz^*\right) \,
    \norm{ \vs\left(\vlambda;\vz^*\right)} \, d\vz^*
    &\leq
    \int \eta\left(\vz\right) \,
    \frac{q\left(\vz\right)}{\pi\left(\vz\right)} \, d\vz \,
    \int \pi\left(\vz^*\right) \,
    \norm{ \vs\left(\vlambda;\vz^*\right)} \, d\vz^*
    \\
    &=
    \Esub{\pi}{\norm{ \vs\left(\vlambda;\vz^*\right)}} \,
    \int \eta\left(\vz\right) \,
    \frac{q\left(\vz\right)}{\pi\left(\vz\right)} \, d\vz \,
    \\
    &=
    \Esub{\pi}{\norm{ \vs\left(\vlambda;\vz^*\right)}} \,
    \int q\left(\vz\right) \, 
    \frac{\eta\left(\vz\right)}{\pi\left(\vz\right)} \, d\vz \,
    \\
    &\leq
    M \,
    \Esub{\pi}{\norm{ \vs\left(\vlambda;\vz^*\right)}}
    \int q\left(\vz\right) \, d\vz \,
    \\
    &=
    M \,
    \Esub{\pi}{\norm{ \vs\left(\vlambda;\vz^*\right)}}.
  \end{align}

  Meanwhile, for T2,
  \begin{align}
      \frac{1}{N} \sum_{n=1}^{N}
        \int \eta\left(\vz\right) \abs{ \lambda^{n}\left( w\left(\vz\right) \right) - \lambda\left( w\left(\vz\right) \right)} \; \norm{\vs\left(\vlambda;\vz\right)} \, d\vz
      &=
      \frac{1}{N} \sum_{n=1}^{N}
        \int \eta\left(\vz\right) \lambda\left( w\left(\vz\right) \right) \, \abs{\lambda^{n-1}\left( w\left(\vz\right) \right) - 1} \; \norm{\vs\left(\vlambda;\vz\right)} \, d\vz
      \\
      &\leq
      \frac{1}{N} \sum_{n=1}^{N}
        \int \eta\left(\vz\right) \lambda\left( w\left(\vz\right) \right) \, \norm{\vs\left(\vlambda;\vz\right)} \, d\vz
      \\
      &=
      \int \eta\left(\vz\right) \lambda\left( w\left(\vz\right) \right) \, \norm{\vs\left(\vlambda;\vz\right)} \, d\vz
      \\
      &\leq
      \left( 1 - \frac{1}{w^*} \right) \,
      \int \eta\left(\vz\right) \, \norm{\vs\left(\vlambda;\vz\right)} \, d\vz
      \\
      &\leq
      \left( 1 - \frac{1}{w^*} \right) \,
      \Esub{\eta}{\norm{\vs\left(\vlambda;\vz\right)}}.
  \end{align}
  Combining T1, T2, T3, and T4, we conclude by
  \begin{align}
    &\abs{
      \text{Bias}\left[\vg_{\text{seq.-IMH}}\right]
      -
      \text{Bias}\left[\vg_{\text{par.-IMH}}\right]
    }   
    \\
    &\leq
    \max\left\{\, n \, {\left(1 - \frac{1}{w^*}\right)}^{n-1} - 1, 1 \,\right\} \,
    \left(\Esub{q}{\norm{\vs\left(\vlambda;\vz\right)}} +  M \, \Esub{\pi}{\norm{ \vs\left(\vlambda;\vz^*\right)}}\right)
    +
      \left( 1 - \frac{1}{w^*} \right) \,
      \Esub{\eta}{\norm{\vs\left(\vlambda;\vz\right)}}.
  \end{align}
\end{proofEnd}

%%% Local Variables:
%%% TeX-master: "master"
%%% End:
