

\textit{Detailed derivation of \textbf{\cref{eq:cis_kernel}}}
\begin{align}
f(\vz) &= \frac{\sum_{i=0}^N w(\vz^{(i)})f(\vz^{(i)})}{\sum_{i=0}^N w(\vz^{(i)})} = \frac{\sum_{i=1}^N w(\vz^{(i)})f(\vz^{(i)}) + w(\vz_{t-1})f(\vz_{t-1})}{\sum_{i=0}^N w(\vz^{(i)})} \\
    &=\frac{\sum_{i=1}^N w(\vz^{(i)})}{\sum_{i=0}^N w(\vz^{(i)})}\frac{\sum_{i=1}^N w(\vz^{(i)})f(\vz^{(i)})}{\sum_{i=1}^N w(\vz^{(i)})} +\frac{w(\vz_{t-1})}{\sum_{i=0}^N w(\vz^{(i)})}f(\vz_{t-1})\\
    &= \alpha(z_{t-1},\vz^{(1:N)})\frac{\sum_{i=1}^N w(\vz^{(i)})f(\vz^{(i)})}{\sum_{i=1}^N w(\vz^{(i)})} + r(z_{t-1}|\vz^{(1:N)})f(\vz_{t-1}),
\end{align}
where
    \(
    \alpha\,(\vz_{t-1}, \vz^{(1:N)}) =
      \sum^{N}_{i=1} w\,(\vz^{(i)})  
    /
      \sum^{N}_{i=0} w\,(\vz^{(i)})  
  \), $f_{IS}=\sum_{i=1}^N w(\vz^{(i)})f(\vz^{(i)})/\sum_{i=1}^N w(\vz^{(i)})$, and 
  \(
  r\,(\vz_{t-1}\mid\vz^{(1:N)}) =w\,(\vz_{t-1}) / \sum^{N}_{i=0} w\,(\vz^{(i)}).
  \)

Taking expectations on both sides, we get
\begin{align}
\mathbb{E}[f(\vz)] &= \mathbb{E}\left[ \alpha(z_{t-1},\vz^{(1:N)})\frac{\sum_{i=1}^N w(\vz^{(i)})f(\vz^{(i)})}{\sum_{i=1}^N w(\vz^{(i)})}\right] + \mathbb{E}[r(z_{t-1}|\vz^{(1:N)})f(z_{t-1})]\\
    &= \mathbb{E}\left[ \alpha(z_{t-1},\vz^{(1:N)})\frac{\sum_{i=1}^N w(\vz^{(i)})f(\vz^{(i)})}{\sum_{i=1}^N w(\vz^{(i)})}\right] + r(\vz_{t-1})f(\vz_{t-1}).
\end{align}

%\\
%
  %% &=  
  %%  \int \alpha\,(\vz_{t-1}, \vz^{(1:N)}) \,
  %%   \frac{
  %%     \sum^{N}_{i=1} w\,(\vz^{(i)})\,f(\vz^{(i)})
  %%   }
  %%   {
  %%     \sum^{N}_{i=1} w\,(\vz^{(i)})
  %%   } \,
  %%   q_{\vlambda}(\vz^{(1:N)})\,d\vz^{(1:N)}
  %%   +
  %%  r\,(\vz_{t-1})\,f(\vz_{t-1})

%%% Local Variables:
%%% TeX-master: "master"
%%% End:
