

\textit{Detailed derivation of \textbf{Equation}~\eqref{eq:cis_kernel}}
\begin{proof}[\unskip\nopunct]
\begin{align}
  &\Esub{K(\vz_{t-1}, \cdot)}{f(\vz)} \\
  &= \Esub{q_{\vlambda}}{
      \sum^{N}_{i=0} w\,(\vz^{(i)}) f(\vz^{(i)}) 
      \,/\,
      \sum^{N}_{i=0} w\,(\vz^{(i)})
  } \\
  \intertext{
    (with a slight abuse of notation \(\vz_{t-1} = \vz^{(0)}\))
  }
  &= \Esub{q_{\vlambda}}{
    \Big(
    \sum^{N}_{i=1} w\,(\vz^{(i)})\,f(\vz^{(i)}) + w\,(\vz_{t-1}) f(\vz_{t-1})
    \Big)
      \,/\,
      \sum^{N}_{i=0} w\,(\vz^{(i)})
  } \\
  &= \Esub{q_{\vlambda}}{
    \frac{
      \sum^{N}_{i=1} w\,(\vz^{(i)})\,f(\vz^{(i)})
    }
    {
      \sum^{N}_{i=0} w\,(\vz^{(i)})
    }
    +
    \frac{w\,(\vz_{t-1})}{\sum^{N}_{i=0} w\,(\vz^{(i)})} f(\vz_{t-1})
  } \\
  &= \Esub{q_{\vlambda}}{
    \frac{
      \sum^{N}_{i=1} w\,(\vz^{(i)})  
    }
    {
      \sum^{N}_{i=0} w\,(\vz^{(i)})  
    }
    \frac{
      \sum^{N}_{i=1} w\,(\vz^{(i)})\,f(\vz^{(i)})
    }
    {
      \sum^{N}_{i=1} w\,(\vz^{(i)})
    }
    +
    \frac{w\,(\vz_{t-1})}{\sum^{N}_{i=0} w\,(\vz^{(i)})} f(\vz_{t-1})
  } \\
  &= \Esub{q_{\vlambda}}{
    \left(
    1 - \frac{
       w\,(\vz_{t-1}) 
    }
    {
      \sum^{N}_{i=0} w\,(\vz^{(i)})  
    }
    \right)\,
    \frac{
      \sum^{N}_{i=1} w\,(\vz^{(i)})\,f(\vz^{(i)})
    }
    {
      \sum^{N}_{i=1} w\,(\vz^{(i)})
    }
    +
    \frac{w\,(\vz_{t-1})}{\sum^{N}_{i=0} w\,(\vz^{(i)})} f(\vz_{t-1})
  } \\
  &= \Esub{q_{\vlambda}}{
    \alpha\,(\vz_{t-1}, \vz^{(1:N)}) \,
    \frac{
      \sum^{N}_{i=1} w\,(\vz^{(i)})\,f(\vz^{(i)})
    }
    {
      \sum^{N}_{i=1} w\,(\vz^{(i)})
    }
    +
    r\,(\vz_{t-1}\mid\vz^{(1:N)}) \, f(\vz_{t-1})
  } \\ 
  \intertext{where we denote
    \(
    \alpha\,(\vz_{t-1}, \vz^{(1:N)}) =
    \frac{
      \sum^{N}_{i=1} w\,(\vz^{(i)})  
    }
    {
      \sum^{N}_{i=0} w\,(\vz^{(i)})  
    }
  \),
  \(
  r\,(\vz_{t-1}\mid\vz^{(1:N)}) = \frac{w\,(\vz_{t-1})}{\sum^{N}_{i=0} w\,(\vz^{(i)})}
  \), and thus,
  }
%
  &= \Esub{q_{\vlambda}}{
    \alpha\,(\vz_{t-1}, \vz^{(1:N)}) \,
    \frac{
      \sum^{N}_{i=1} w\,(\vz^{(i)})\,f(\vz^{(i)})
    }
    {
      \sum^{N}_{i=1} w\,(\vz^{(i)})
    }
  }
    +
 \Esub{q_{\vlambda}}{
   r\,(\vz_{t-1}\mid\vz^{(1:N)})
 } f(\vz_{t-1}) \\
%
  &= \Esub{q_{\vlambda}}{
    \alpha\,(\vz_{t-1}, \vz^{(1:N)}) \,
    \frac{
      \sum^{N}_{i=1} w\,(\vz^{(i)})\,f(\vz^{(i)})
    }
    {
      \sum^{N}_{i=1} w\,(\vz^{(i)})
    }
  }
    +
   r\,(\vz_{t-1})\,f(\vz_{t-1}) %\\
%
  %% &=  
  %%  \int \alpha\,(\vz_{t-1}, \vz^{(1:N)}) \,
  %%   \frac{
  %%     \sum^{N}_{i=1} w\,(\vz^{(i)})\,f(\vz^{(i)})
  %%   }
  %%   {
  %%     \sum^{N}_{i=1} w\,(\vz^{(i)})
  %%   } \,
  %%   q_{\vlambda}(\vz^{(1:N)})\,d\vz^{(1:N)}
  %%   +
  %%  r\,(\vz_{t-1})\,f(\vz_{t-1})
\end{align}
\end{proof}

%%% Local Variables:
%%% TeX-master: "master"
%%% End:
